Test/Api/ApiContract.lean
@@ -1,4 +1,5 @@
 import Test.Api.ExternalContract
+import Test.Api.PackagesContract
 import Effect4.Api
 import TypeScript.Render
 
